src/OeufProof.v
@@ -29,6 +29,8 @@ Require Dmajortodflatmajor.
 Require Dflatmajortocmajor.
 Require Cmajortominor.
 
+Require Import Cmajor. (* Cminor bridge *)
+Require Import OeufCompcertSimulations.
 
 Require Import compcert.lib.Coqlib.
 Require Import compcert.ia32.Asm.
@@ -53,7 +55,7 @@ Section Simulation.
   (* In this theorem we grab all of the things we need from all of the passes *)
   Theorem Oeuf_forward_simulation :
     forall ty,
-      mix_forward_simulation (@CompilationUnit.source_semantics ty prog) (Asm.semantics tprog).
+      mix_forward_simulation (@CompilationUnit.source_semantics ty prog) (Cminor_semantics tprog).
   Proof.
     (* SourceLang to Untyped *)
     unfold transf_to_asm in TRANSF.
